metatheory/typeSoundScript.sml
@@ -11,26 +11,6 @@ open typeSoundInvariantsTheory evalPropsTheory;
 
 val _ = new_theory "typeSound";
 
-val merge_envC_assoc = Q.store_thm ("merge_envC_assoc",
-`∀envC1 envC2 envC3.
-  merge_envC envC1 (merge_envC envC2 envC3) =
-  merge_envC (merge_envC envC1 envC2) envC3`,
-rw [] >>
-PairCases_on `envC1` >>
-PairCases_on `envC2` >>
-PairCases_on `envC3` >>
-rw [merge_envC_def, merge_def]);
-
-val merge_tenvC_assoc = Q.store_thm ("merge_tenvC_assoc",
-`∀tenvC1 tenvC2 tenvC3.
-  merge_tenvC tenvC1 (merge_tenvC tenvC2 tenvC3) =
-  merge_tenvC (merge_tenvC tenvC1 tenvC2) tenvC3`,
-rw [] >>
-PairCases_on `tenvC1` >>
-PairCases_on `tenvC2` >>
-PairCases_on `tenvC3` >>
-rw [merge_tenvC_def, merge_def])
-
 val union_decls_empty = Q.store_thm ("union_decls_empty",
 `!decls. union_decls empty_decls decls = decls`,
  rw [] >>
